demo/union_find/UnionFindSource.v
@@ -7,7 +7,7 @@ Require Export Simulation.
 Require Import Skeleton Mod ModSem.
 Require ClightC.
 Require Import UnionFindTarget.
-Require Import SIR.
+Require Import SIR3.
 
 (* Require Import Clightdefs. *)
 
@@ -102,7 +102,7 @@ Definition c_unionS (vs: list val): itree (E owned_heap) val := triggerUB "".
 Definition f_unionS: function owned_heap :=
   mkfunction (ClightC.signature_of_function f_unionS) c_unionS.
 
-Definition global_definitions: list (ident * globdef (fundef (SIR.function owned_heap)) unit) :=
+Definition global_definitions: list (ident * globdef (fundef (function owned_heap)) unit) :=
 ((_malloc, Gfun(External EF_malloc)) ::
  (_makeSet, Gfun(Internal f_makeSet)) :: (_find, Gfun(Internal f_find)) ::
  (_unionS, Gfun(Internal f_unionS)) ::
@@ -111,9 +111,9 @@ Definition global_definitions: list (ident * globdef (fundef (SIR.function owned
 )
 .
 
-Definition prog: SIR.program owned_heap := mkprogram global_definitions public_idents _main.
+Definition prog: program owned_heap := mkprogram global_definitions public_idents _main.
 
-Definition module: Mod.t := SIR.module prog "UF"%string initial_owned_heap.
+Definition module: Mod.t := module prog "UF"%string initial_owned_heap.
 
 (* void unionS(struct Node* x, struct Node* y) { *)
 (*   struct Node *xRoot, *yRoot; *)
